---
title: "Untitled"
format: html
editor: visual
---

# Exercise 3 - solution

Firrst of all:

$$
7-MA_t = \frac{1}{7}\sum_{j=-3}^{j=+3}y_{t+j} = \frac{1}{7}(y_{t-3}+y_{t-2}+y_{t-1}+y_{t}+y_{t+11}+y_{t+2}+y_{t+3})
$$

on the other hand:

$$
3\times7-MA_t = \frac{1}{3}(7-MA_{t-1}+7-MA_{t}+7-MA_{t+1}) = \cdots = 
$$

Develop the formula to reach the final solution.

# Exercise 4 - solution

Firrst of all:

$$
8-MA_t = \frac{1}{8}\sum_{j=-3}^{j=+4}y_{t+j} = \frac{1}{8}(y_{t-3}+y_{t-2}+y_{t-1}+y_{t}+y_{t+1}+y_{t+2}+y_{t+3}+y_{t+4})
$$

subsequent averaging to have an overall centered window:

$$
2\times8-MA_t = \frac{1}{2}(8-MA_{t-1}+8-MA_{t}) = \cdots = 
$$

Alternatively:

$$
8-MA_t = \frac{1}{8}\sum_{j=-3}^{j=+4}y_{t+j} = \frac{1}{8}(y_{t-4}+y_{t-3}+y_{t-2}+y_{t-1}+y_{t}+y_{t+1}+y_{t+2}+y_{t+3})
$$

and accordingly, averaging again to have an overall centered window:

$$
2\times8-MA_t = \frac{1}{2}(8-MA_{t}+8-MA_{t+1}) = \cdots = 
$$

The same result should be reached in both instances.